Removing accumulate_freshness assumptions

secure_api/aead/Crypto.AEAD.Encoding.fst
@@ -44,9 +44,6 @@ type txtlen_32 = l:UInt32.t {l <=^ txtmax}
 //16-09-18 where is it in the libraries?
 private let min (a:nat) (b:nat) : nat = if a <= b then a else b
 
-//val lemma_append_nil: #a:_ -> s:Seq.seq a -> Lemma (s == Seq.append s Seq.createEmpty)
-//let lemma_append_nil #a s = assert (Seq.equal s (Seq.append s Seq.createEmpty))
-
 
 (* * *********************************************)
 (* *            Encoding                         *)
@@ -393,8 +390,14 @@ let lemma_encode_both_inj i (al0:aadlen_32) (pl0:txtlen_32) (al1:aadlen_32) (pl1
   lemma_encode_bytes_injective p0 p1;
   lemma_encode_bytes_injective a0 a1
 
+
+let fresh_sref (#a:Type0) h0 h1 (r:HS.reference a) = 
+  ~(h0 `HS.contains` r) /\
+  HS.frameOf r == HS.(h1.tip) /\
+  h1 `HS.contains` r
+
 val accumulate: 
-  #i: MAC.id -> st: CMA.state i -> 
+  #i:MAC.id -> st:CMA.state i ->
   aadlen:aadlen_32 -> aad:lbuffer (v aadlen) ->
   txtlen:txtlen_32 -> cipher:lbuffer (v txtlen) -> 
   StackInline (CMA.accBuffer i)   // StackInline required for stack-allocated accumulator
@@ -405,29 +408,29 @@ val accumulate:
     Buffer.disjoint_2 CMA.(MAC.as_buffer st.r) aad cipher))
   (ensures (fun h0 a h1 -> 
     Buffer.modifies_0 h0 h1 /\ // modifies only fresh buffers on the current stack
-    ~ (h0 `Buffer.contains` CMA.(MAC.as_buffer (abuf a))) /\
-    Buffer.live h1 aad /\ 
+    // fresh_sref h0 h1 (Buffer.content (MAC.as_buffer (CMA.abuf a))) /\
+    ~ (h0 `Buffer.contains` (MAC.as_buffer (CMA.abuf a))) /\
+    Buffer.frameOf (MAC.as_buffer (CMA.abuf a)) == h1.tip /\
+    Buffer.live h1 aad /\
     Buffer.live h1 cipher /\
-    Buffer.frameOf CMA.(MAC.as_buffer (abuf a)) = h1.tip /\
     CMA.acc_inv st a h1 /\
     (if mac_log then
-        let log = CMA.alog a in
-        //16-12-15 settle for a weaker property? modifies_nothing h0 h1 /\ 
-        FStar.HyperStack.sel h1 log == encode_both (fst i) aadlen (Buffer.as_seq h1 aad) txtlen (Buffer.as_seq h1 cipher)
-      else
-        Buffer.modifies_0 h0 h1)))
+       let log = CMA.alog a in
+       fresh_sref h0 h1 log /\
+       //16-12-15 settle for a weaker property? modifies_nothing h0 h1 /\
+       HS.sel h1 log ==
+       encode_both (fst i) aadlen (Buffer.as_seq h1 aad) txtlen (Buffer.as_seq h1 cipher)
+     else
+       Buffer.modifies_0 h0 h1)))
 
-val lemma_append_nil: #a:_ -> s:Seq.seq a -> Lemma (s == Seq.append s Seq.createEmpty)
-let lemma_append_nil #a s = assert (Seq.equal s (Seq.append s Seq.createEmpty))
- 
-#reset-options "--initial_fuel 0 --max_fuel 0 --initial_ifuel 0 --max_ifuel 0 --z3rlimit 200"
-let accumulate #i st aadlen aad txtlen cipher  = 
+#reset-options "--initial_fuel 0 --max_fuel 0 --initial_ifuel 0 --max_ifuel 0 --z3rlimit 2000"
+let accumulate #i st aadlen aad txtlen cipher  =
   let h = ST.get() in 
   let acc = CMA.start st in
   let h0 = ST.get() in
-  //assert(mac_log ==> h0 `contains` (CMA.alog acc));
+  assert (mac_log ==> fresh_sref h h0 (CMA.alog acc));
   Buffer.lemma_reveal_modifies_0 h h0;
-  //assert (Buffer.disjoint_2 (MAC.as_buffer (CMA.(abuf acc))) aad cipher);
+  assert (Buffer.disjoint_2 (MAC.as_buffer (CMA.(abuf acc))) aad cipher);
   add_bytes st acc aadlen aad;
   let h1 = ST.get() in 
   add_bytes st acc txtlen cipher;
@@ -435,32 +438,31 @@ let accumulate #i st aadlen aad txtlen cipher  =
   let final_word = Buffer.create 0uy 16ul in 
   let h3 = ST.get() in
   Buffer.lemma_reveal_modifies_0 h2 h3;
-  //assert(mac_log ==> h3 `contains` (CMA.alog acc)); 
+  assert(mac_log ==> h3 `contains` (CMA.alog acc));
   let id, _ = i in  // JP: removed a call to Prims.fst
-  ( match macAlg_of_id id with 
+  (match macAlg_of_id id with
     | POLY1305 -> store_lengths_poly1305 aadlen txtlen final_word
-    | GHASH -> store_lengths_ghash aadlen txtlen final_word );
+    | GHASH    -> store_lengths_ghash    aadlen txtlen final_word);
   let h4 = ST.get() in 
   Buffer.lemma_reveal_modifies_1 final_word h3 h4;
   CMA.frame_acc_inv st acc h2 h3;
   CMA.frame_acc_inv st acc h3 h4;
   CMA.update st acc final_word;
-  let h5 = ST.get() in 
-
+  let h5 = ST.get() in
   if mac_log then 
     begin
       let open FStar.Seq in 
       let al = CMA.alog acc in
+      assert (fresh_sref h h5 al);
       let cbytes = Buffer.as_seq h cipher in 
       let abytes = Buffer.as_seq h aad in 
       let lbytes = Buffer.as_seq h4 final_word in 
       assert(equal (HS.sel h0 al) createEmpty);
-      lemma_append_nil (encode_bytes abytes);
+      Seq.append_empty_r (encode_bytes abytes);
       assert(equal (HS.sel h1 al) (encode_bytes abytes));
       assert(equal (HS.sel h2 al) (encode_bytes cbytes @| encode_bytes abytes));
       assert(equal (HS.sel h5 al) (Seq.cons lbytes (encode_bytes cbytes @| encode_bytes abytes)));
       assert(equal (HS.sel h5 al) (encode_both (fst i) aadlen abytes txtlen cbytes));
-
       assert(HS.modifies_one h.tip h h0);
       assert(HS.modifies_one h.tip h0 h2);
       assert(HS.modifies_one h.tip h2 h3);
